cleanup

theories/crypto/ICCA.ec
@@ -112,10 +112,9 @@ module Ideal : ICCA_Oracle = {
   }
 }.
 
-module Ideal' : ICCA_Oracle = {
+module IdealS : ICCA_Oracle = {
   import var Real
-  var n : int
-  var cs : (int * (ciphertext * plaintext)) list
+  var cs : (ciphertext * plaintext) list
 
   proc init() : unit = {
     var ks;
@@ -123,7 +122,6 @@ module Ideal' : ICCA_Oracle = {
     ks <$ dkeyseed;
     pk <- pkgen ks;
     sk <- skgen ks;
-    n <- 0;
     cs <- [];
   }
 
@@ -136,18 +134,17 @@ module Ideal' : ICCA_Oracle = {
 
     e <$ dencseed;
     c <- enc(m0, pk, e);
-    n <- n + 1;
-    cs <- (n, (c, m)) :: cs;
+    cs <- (c, m) :: cs;
     return c;
   }
 
   proc dec (c : ciphertext) : plaintext option = {
     var fcs, m, p;
 
-    fcs <- List.filter (fun p => fst (snd p) = c) cs;
+    fcs <- List.filter (fun p => fst p = c) cs;
     if (fcs <> []) {
       p <$ drat fcs;
-      m <- Some (snd (snd p));
+      m <- Some (snd p);
     } else {
       m <- dec(c, sk);
     }
@@ -192,9 +189,9 @@ module Real' : ICCA_Oracle = {
   }
 }.
 
-module Real'' : ICCA_Oracle = {
+module RealS' : ICCA_Oracle = {
   import var Real
-  import var Ideal'
+  import var IdealS
 
   proc init() : unit = {
     var ks;
@@ -202,7 +199,6 @@ module Real'' : ICCA_Oracle = {
     ks <$ dkeyseed;
     pk <- pkgen ks;
     sk <- skgen ks;
-    n <- 0;
     cs <- [];
   }
 
@@ -215,18 +211,17 @@ module Real'' : ICCA_Oracle = {
 
     e <$ dencseed;
     c <- enc(m, pk, e);
-    n <- n + 1;
-    cs <- (n, (c, m)) :: cs;
+    cs <- (c, m) :: cs;
     return c;
   }
 
   proc dec (c : ciphertext) : plaintext option = {
     var fcs, m, p;
 
-    fcs <- List.filter (fun p => fst (snd p) = c) cs;
+    fcs <- List.filter (fun p => fst p = c) cs;
     if (fcs <> []) {
       p <$ drat fcs;
-      m <- Some (snd (snd p));
+      m <- Some (snd p);
     } else {
       m <- dec(c, sk);
     }
@@ -327,9 +322,8 @@ module B (A : Adversary) (O : CCA_Oracle) = {
   }
 }.
 
-module B' (A : Adversary) (O : CCA_Oracle) = {
-  var n : int
-  var cs : (int * (ciphertext * plaintext)) list
+module BS (A : Adversary) (O : CCA_Oracle) = {
+  var cs : (ciphertext * plaintext) list
   var pk : pkey
 
   module O' : ICCA_Oracle = {
@@ -342,18 +336,17 @@ module B' (A : Adversary) (O : CCA_Oracle) = {
       var c;
 
       c <- O.l_or_r(m, m0);
-      n <- n + 1;
-      cs <- (n, (c, m)) :: cs;
+      cs <- (c, m) :: cs;
       return c;
     }
 
     proc dec (c : ciphertext) : plaintext option = {
       var fcs, m, p;
 
-      fcs <- List.filter (fun p => fst (snd p) = c) cs;
+      fcs <- List.filter (fun p => fst p = c) cs;
       if (fcs <> []) {
         p <$ drat fcs;
-        m <- Some (snd (snd p));
+        m <- Some (snd p);
       } else {
         m <- O.dec(c);
       }
@@ -364,7 +357,6 @@ module B' (A : Adversary) (O : CCA_Oracle) = {
   proc main (pk : pkey) : bool = {
     var r;
 
-    n <- 0;
     cs <- [];
     O'.init(pk);
     r <@ A(O').main();
@@ -374,7 +366,34 @@ module B' (A : Adversary) (O : CCA_Oracle) = {
 
 section.
 
-declare module A : Adversary {Real, Real', Ideal, Ideal', C.Wrap, B, B', CountCCA, CountICCA}.
+declare module A : Adversary {Real, Real', Ideal, IdealS,
+                              C.Wrap, B, BS, CountCCA, CountICCA}.
+
+module S : Scheme = {
+  proc kg () : pkey * skey = {
+    var ks, pk, sk;
+
+    ks <$ dkeyseed;
+    pk <- pkgen ks;
+    sk <- skgen ks;
+    return (pk, sk);
+  }
+
+  proc enc (pk : pkey, m : plaintext) : ciphertext = {
+    var e, c;
+
+    e <$ dencseed;
+    c <- enc (m, pk, e);
+    return c;
+  }
+
+  proc dec(sk : skey, c : ciphertext) : plaintext option = {
+    var m;
+
+    m <- dec (c, sk);
+    return m;
+  }
+}.
 
 axiom A_bound (O <: ICCA_Oracle {A, CountICCA}) : hoare [CountAdv(A, O).main :
                true ==> CountICCA.ndec <= Ndec /\ CountICCA.nenc <= Nenc].
@@ -405,67 +424,24 @@ equiv Real_Real' :
   Game(Real, A).main ~ Game(Real', A).main : ={glob A} ==> ={res}.
 proof.
 proc; inline *.
-call (: ={glob Real} /\ (exists ks, (Real.pk, Real.sk){2} = (pkgen ks, skgen ks)) /\
+call (: ={glob Real} /\
+        (exists ks, (Real.pk, Real.sk){2} = (pkgen ks, skgen ks)) /\
         (forall c m, assoc Ideal.cs c = Some m => dec(c, Real.sk) = Some m){2}).
 - by proc; auto.
 - proc; wp; rnd; auto=> /> &m2 ks Hcs e _ c m'.
-  rewrite assoc_cons. case: (c = enc (m{m2}, pkgen ks, e)) => />; 1: by rewrite encK.
+  rewrite assoc_cons.
+  case: (c = enc (m{m2}, pkgen ks, e)) => />; 1: by rewrite encK.
   by move => _; apply: Hcs.
 - by proc; wp; skip => /> &m2 ks Hcs /#.
 - by wp; rnd; skip => /> /#.
 qed.
-
-equiv Real_Real'' :
-  Game(Real, A).main ~ Game(Real'', A).main : ={glob A} ==> ={res}.
-proof.
-proc; inline *.
-call (: ={glob Real} /\ (exists ks, (Real.pk, Real.sk){2} = (pkgen ks, skgen ks)) /\
-        (forall c p, p \in drat (List.filter (fun p => fst (snd p) = c) Ideal'.cs) =>
-                     dec(c, Real.sk) = Some (snd (snd p))){2}).
-- by proc; auto.
-- proc; wp; rnd; auto => /> &m2 ks csP e ? c ?.
-  case: (enc (m{m2}, pkgen ks, e) = c); 2: by move => _; apply csP.
-  rewrite supp_drat in_cons.
-  move => ? [|]; 1: smt(encK).
-  by rewrite -supp_drat; apply csP.
-- proc; sp; if{2}; 2: by auto => />.
-  auto => /> &m2 ks Hcs fP; split; 1: smt(drat_ll).
-  by move => _; apply Hcs.
-- by wp; rnd; skip => />; smt(supp_drat).
-qed.
-
-module S : Scheme = {
-  proc kg () : pkey * skey = {
-    var ks, pk, sk;
-
-    ks <$ dkeyseed;
-    pk <- pkgen ks;
-    sk <- skgen ks;
-    return (pk, sk);
-  }
-
-  proc enc (pk : pkey, m : plaintext) : ciphertext = {
-    var e, c;
-
-    e <$ dencseed;
-    c <- enc (m, pk, e);
-    return c;
-  }
-
-  proc dec(sk : skey, c : ciphertext) : plaintext option = {
-    var m;
-
-    m <- dec (c, sk);
-    return m;
-  }
-}.
 
 equiv Real'_CCA_L :
   Game(Real', A).main ~ CCA_L(S, B(A)).main : ={glob A} ==> ={res}.
 proof.
 proc; inline *; wp.
 call (: ={pk, sk}(Real, Wrap) /\ unzip1 Ideal.cs{1} = Wrap.cs{2} /\
-        (forall c m, assoc Ideal.cs c = Some m => dec(c, Real.sk) = Some m){1} /\
+        (forall c m,assoc Ideal.cs c = Some m => dec(c, Real.sk) = Some m){1} /\
         (exists ks, (Wrap.pk, Wrap.sk){2} = (pkgen ks, skgen ks)) /\
         Ideal.cs{1} = B.cs{2} /\ B.pk{2} = Wrap.pk{2}).
 - by proc; inline *; auto => />.
@@ -476,35 +452,13 @@ call (: ={pk, sk}(Real, Wrap) /\ unzip1 Ideal.cs{1} = Wrap.cs{2} /\
 - by wp; rnd; skip => /> /#.
 qed.
 
-equiv Real''_CCA_L :
-  Game(Real'', A).main ~ CCA_L(S, B'(A)).main : ={glob A} ==> ={res}.
-proof.
-proc; inline *; wp.
-call (: ={pk, sk}(Real,Wrap) /\ unzip1 (unzip2 Ideal'.cs{1}) = Wrap.cs{2} /\
-        (forall c i m, (i, (c, m)) \in List.filter (fun p => fst (snd p) = c)
-                                                   Ideal'.cs =>
-                       dec(c, Real.sk) = Some m){1} /\
-        (exists ks, (Wrap.pk, Wrap.sk){2} = (pkgen ks, skgen ks)) /\
-        Ideal'.cs{1} = B'.cs{2} /\ B'.pk{2} = Wrap.pk{2} /\
-        Ideal'.n{1} = B'.n{2}).
-- by proc; inline *; auto => />.
-- proc; inline *; auto => /> &m1 &m2 Hcs ks skP ? e _ c i ?.
-  case: (enc (m{m2}, pkgen ks, e) = c).
-  + move => ? [|?]; 1: smt(encK).
-    by rewrite -skP; apply (Hcs c i); smt().
-  + by move => _ ?; rewrite -skP; apply (Hcs c i); smt().
-- proc; inline *; sp; auto; if; auto => /> &m1 &m2 Hcs ks ? ? csP.
-  rewrite mem_map_fst; move => [?].
-  rewrite mem_map_snd; smt(mem_filter).
-- by wp; rnd; skip => /> /#.
-qed.
-
 equiv Ideal_CCA_R :
   Game(Ideal, A).main ~ CCA_R(S, B(A)).main : ={glob A} ==> ={res}.
 proof.
 proc; inline *; wp.
-call (: ={pk, sk}(Real,Wrap) /\ unzip1 Ideal.cs{1} = Wrap.cs{2} /\
-        (forall c m, assoc Ideal.cs c = Some m => dec(c, Real.sk) = Some m0){1} /\
+call (: ={pk, sk}(Real, Wrap) /\ unzip1 Ideal.cs{1} = Wrap.cs{2} /\
+        (forall c m,
+           assoc Ideal.cs c = Some m => dec(c, Real.sk) = Some m0){1} /\
         (exists ks, (Wrap.pk, Wrap.sk){2} = (pkgen ks, skgen ks)) /\
         Ideal.cs{1} = B.cs{2} /\ B.pk{2} = Wrap.pk{2}).
 - by proc; inline *; auto => />.
@@ -515,49 +469,94 @@ call (: ={pk, sk}(Real,Wrap) /\ unzip1 Ideal.cs{1} = Wrap.cs{2} /\
 - by wp; rnd; skip => /> /#.
 qed.
 
-equiv Ideal'_CCA_R :
-  Game(Ideal', A).main ~ CCA_R(S, B'(A)).main : ={glob A} ==> ={res}.
-proof.
-proc; inline *; wp.
-call (: ={pk, sk}(Real,Wrap) /\ unzip1 (unzip2 Ideal'.cs{1}) = Wrap.cs{2} /\
-        (forall c i m, (i, (c, m)) \in List.filter (fun p => fst (snd p) = c)
-                                                   Ideal'.cs =>
-                       dec(c, Real.sk) = Some m0){1} /\
-        (exists ks, (Wrap.pk, Wrap.sk){2} = (pkgen ks, skgen ks)) /\
-        Ideal'.cs{1} = B'.cs{2} /\ B'.pk{2} = Wrap.pk{2} /\
-        Ideal'.n{1} = B'.n{2}).
-- by proc; inline *; auto => />.
-- proc; inline *; auto => /> &m1 &m2 Hcs ks skP ? e _ c i m'.
-  case: (enc (m0, pkgen ks, e) = c); 1: smt(encK).
-  by move => _ ?; rewrite -skP; apply (Hcs c i m'); smt().
-- proc; inline *; sp; auto; if; auto => /> &m1 &m2 Hcs ks ? ? csP.
-  rewrite mem_map_fst; move => [?].
-  rewrite mem_map_snd; smt(mem_filter).
-- by wp; rnd; skip => /> /#.
-qed.
-
 lemma ICCA_CCALR &m :
   Pr[Game(Real, A).main() @ &m : res] - Pr[Game(Ideal, A).main() @ &m : res] =
   Pr[CCA_L(S, B(A)).main() @ &m : res] - Pr[CCA_R(S, B(A)).main() @ &m : res].
 proof.
-have -> : Pr[Game(Real, A).main() @ &m : res] = Pr[Game(Real', A).main() @ &m : res].
+have -> : Pr[Game(Real, A).main() @ &m : res] =
+          Pr[Game(Real', A).main() @ &m : res].
 - byequiv => //; conseq (: ={glob A} ==> ={res}) => //; exact Real_Real'.
-have -> : Pr[Game(Real', A).main() @ &m : res] = Pr[CCA_L(S, B(A)).main() @ &m : res].
+have -> : Pr[Game(Real', A).main() @ &m : res] =
+          Pr[CCA_L(S, B(A)).main() @ &m : res].
 - byequiv => //; conseq (: ={glob A} ==> ={res}) => //; exact Real'_CCA_L.
-have -> : Pr[Game(Ideal, A).main() @ &m : res] = Pr[CCA_R(S, B(A)).main() @ &m : res]; 2: by smt().
+have -> : Pr[Game(Ideal, A).main() @ &m : res] =
+          Pr[CCA_R(S, B(A)).main() @ &m : res]; 2: by smt().
 byequiv => //; conseq (: ={glob A} ==> ={res}) => //; exact Ideal_CCA_R.
 qed.
 
-lemma ICCA_CCALR' &m :
-  Pr[Game(Real, A).main() @ &m : res] - Pr[Game(Ideal', A).main() @ &m : res] =
-  Pr[CCA_L(S, B'(A)).main() @ &m : res] - Pr[CCA_R(S, B'(A)).main() @ &m : res].
+equiv Real_RealS' :
+  Game(Real, A).main ~ Game(RealS', A).main : ={glob A} ==> ={res}.
 proof.
-have -> : Pr[Game(Real, A).main() @ &m : res] = Pr[Game(Real'', A).main() @ &m : res].
-- byequiv => //; conseq (: ={glob A} ==> ={res}) => //; exact Real_Real''.
-have -> : Pr[Game(Real'', A).main() @ &m : res] = Pr[CCA_L(S, B'(A)).main() @ &m : res].
-- byequiv => //; conseq (: ={glob A} ==> ={res}) => //; exact Real''_CCA_L.
-have -> : Pr[Game(Ideal', A).main() @ &m : res] = Pr[CCA_R(S, B'(A)).main() @ &m : res]; 2: by smt().
-byequiv => //; conseq (: ={glob A} ==> ={res}) => //; exact Ideal'_CCA_R.
+proc; inline *.
+call (: ={glob Real} /\
+        (exists ks, (Real.pk, Real.sk){2} = (pkgen ks, skgen ks)) /\
+        (forall c p,
+           p \in drat (List.filter (fun p => fst p = c) IdealS.cs) =>
+           dec(c, Real.sk) = Some (snd p)){2}).
+- by proc; auto.
+- proc; wp; rnd; auto => /> &m2 ks csP e ? c ?.
+  case: (enc (m{m2}, pkgen ks, e) = c); 2: by move => _; apply csP.
+  rewrite supp_drat in_cons.
+  move => ? [|]; 1: smt(encK).
+  by rewrite -supp_drat; apply csP.
+- proc; sp; if{2}; 2: by auto => />.
+  auto => /> &m2 ? Hcs ?; split; 1: smt(drat_ll).
+  by move => _; apply Hcs.
+- by wp; rnd; skip => />; smt(supp_drat).
+qed.
+
+equiv RealS'_CCA_L :
+  Game(RealS', A).main ~ CCA_L(S, BS(A)).main : ={glob A} ==> ={res}.
+proof.
+proc; inline *; wp.
+call (: ={pk, sk}(Real, Wrap) /\ unzip1 IdealS.cs{1} = Wrap.cs{2} /\
+        (forall c m, (c, m) \in List.filter (fun p => fst p = c) IdealS.cs =>
+                       dec(c, Real.sk) = Some m){1} /\
+        (exists ks, (Wrap.pk, Wrap.sk){2} = (pkgen ks, skgen ks)) /\
+        IdealS.cs{1} = BS.cs{2} /\ BS.pk{2} = Wrap.pk{2}).
+- by proc; inline *; auto => />.
+- proc; inline *; auto => /> &m1 &m2 Hcs ks skP ? e _ c ?.
+  case: (enc (m{m2}, pkgen ks, e) = c).
+  + move => ? [|?]; 1: smt(encK).
+    by rewrite -skP; apply (Hcs c); smt().
+  + by move => _ ?; rewrite -skP; apply (Hcs c); smt().
+- proc; inline *; sp; auto; if; auto => /> &m1 &m2 5?.
+  rewrite mem_map_fst; smt(mem_filter).
+- by wp; rnd; skip => /> /#.
+qed.
+
+equiv IdealS_CCA_R :
+  Game(IdealS, A).main ~ CCA_R(S, BS(A)).main : ={glob A} ==> ={res}.
+proof.
+proc; inline *; wp.
+call (: ={pk, sk}(Real, Wrap) /\ unzip1 IdealS.cs{1} = Wrap.cs{2} /\
+        (forall c m, (c, m) \in List.filter (fun p => fst p = c)
+                                                   IdealS.cs =>
+                       dec(c, Real.sk) = Some m0){1} /\
+        (exists ks, (Wrap.pk, Wrap.sk){2} = (pkgen ks, skgen ks)) /\
+        IdealS.cs{1} = BS.cs{2} /\ BS.pk{2} = Wrap.pk{2}).
+- by proc; inline *; auto => />.
+- proc; inline *; auto => /> &m1 &m2 Hcs ks skP ? e _ c m'.
+  case: (enc (m0, pkgen ks, e) = c); 1: smt(encK).
+  by move => _ ?; rewrite -skP; apply (Hcs c m'); smt().
+- proc; inline *; sp; auto; if; auto => /> &m1 &m2 5?.
+  rewrite mem_map_fst; smt(mem_filter).
+- by wp; rnd; skip => /> /#.
+qed.
+
+lemma ICCA_CCALR' &m :
+  Pr[Game(Real, A).main() @ &m : res] - Pr[Game(IdealS, A).main() @ &m : res] =
+  Pr[CCA_L(S, BS(A)).main() @ &m : res] - Pr[CCA_R(S, BS(A)).main() @ &m : res].
+proof.
+have -> : Pr[Game(Real, A).main() @ &m : res] =
+          Pr[Game(RealS', A).main() @ &m : res].
+- byequiv => //; conseq (: ={glob A} ==> ={res}) => //; exact Real_RealS'.
+have -> : Pr[Game(RealS', A).main() @ &m : res] =
+          Pr[CCA_L(S, BS(A)).main() @ &m : res].
+- byequiv => //; conseq (: ={glob A} ==> ={res}) => //; exact RealS'_CCA_L.
+have -> : Pr[Game(IdealS, A).main() @ &m : res] =
+          Pr[CCA_R(S, BS(A)).main() @ &m : res]; 2: by smt().
+byequiv => //; conseq (: ={glob A} ==> ={res}) => //; exact IdealS_CCA_R.
 qed.
 
 end section.
